existentials

polymorphic-burger-2/systemf.sig
@@ -5,13 +5,15 @@ vl : Type
 bool : ty
 arr : ty -> ty -> ty
 all : (bind ty in ty) -> ty
-exist : (bind ty in ty) -> ty
+ex : (bind ty in ty) -> ty
 
 app  : tm -> tm -> tm
 tapp : tm -> ty -> tm
 vt   : vl -> tm
+unpack : tm -> (bind ty, vl in tm) -> tm
 
 true : vl
 false : vl
 lam  : ty -> (bind vl in tm) -> vl
 tlam : (bind ty in tm) -> vl
+pack : ty -> vl -> vl
